src/Parsers/Examples/ABStar.v
@@ -1,0 +1,104 @@
+(** * Simplified parser for (ab)* *)
+Require Import Coq.Lists.List Coq.Strings.String.
+Require Import Parsers.ContextFreeGrammar.
+Require Import Parsers.BaseTypes Parsers.BooleanBaseTypes.
+Require Import Parsers.Splitters.RDPList.
+Require Import Common.
+
+Require Import Parsers.MinimalParse.
+Require Import Parsers.ContextFreeGrammarNotations.
+Require Import Parsers.Grammars.ABStar.
+
+Require Import Parsers.BooleanRecognizer Parsers.BooleanRecognizerCorrect Parsers.Splitters.FirstChar Parsers.ContextFreeGrammarProperties.
+
+Set Implicit Arguments.
+Local Open Scope string_scope.
+Local Open Scope string_like_scope.
+
+Local Coercion is_true : bool >-> Sortclass.
+Local Notation StringT := (StringWithSplitState string_stringlike (fun _ => True)).
+
+Local Coercion StringT_of_string : string >-> StringWithSplitState.
+
+Section on_ab_star.
+  Definition parse (str : string) : bool
+    := let data := ab_star_data in parse_nonterminal (G := ab_star_grammar) str ab_star_grammar.
+
+  Local Notation correct_parse_T
+    := ({ parse : string -> bool
+                            & forall str,
+                                (parse str -> parse_of_item string_stringlike ab_star_grammar str (NonTerminal _ ab_star_grammar))
+                                * (forall p : parse_of string_stringlike ab_star_grammar str (Lookup ab_star_grammar ab_star_grammar),
+                                     Forall_parse_of_item
+                                       (fun _ nt => is_valid_nonterminal initial_nonterminals_data nt)
+                                       (ParseNonTerminal _ p)
+                                     -> parse_nonterminal (G := ab_star_grammar) str ab_star_grammar) }) (only parsing).
+
+  Definition parse_with_correct
+  : correct_parse_T.
+  Proof.
+    exists parse.
+    exact (fun str => @parse_nonterminal_correct _ _ _ ab_star_cdata str ab_star_grammar).
+  Defined.
+
+  Local Opaque string_dec.
+
+  Definition simplified_parse_with_correct
+  : correct_parse_T.
+  Proof.
+    pose parse_with_correct as p.
+    unfold parse_with_correct in p.
+    Notation "( x ; *** )" := (existT _ x _).
+    unfold parse, parse_nonterminal, parse_nonterminal_or_abort, parse_nonterminal_step, parse_productions, parse_production in p.
+    simpl in p.
+  Abort.
+
+  Definition simplified_parse (str : string) : bool.
+  Proof.
+    pose (parse str) as p.
+    unfold parse, parse_nonterminal, parse_nonterminal_or_abort, parse_nonterminal_step, parse_productions in p.
+    simpl in p.
+    unfold parse in p.
+  Abort.
+End on_ab_star.
+
+Section on_ab_star'.
+  Definition parse' (str : string) : bool
+    := let data := ab_star'_data in parse_nonterminal (G := ab_star_grammar') str ab_star_grammar'.
+
+  Local Notation correct_parse_T
+    := ({ parse : string -> bool
+                            & forall str,
+                                (parse str -> parse_of_item string_stringlike ab_star_grammar' str (NonTerminal _ ab_star_grammar'))
+                                * (forall p : parse_of string_stringlike ab_star_grammar' str (Lookup ab_star_grammar' ab_star_grammar'),
+                                     Forall_parse_of_item
+                                       (fun _ nt => is_valid_nonterminal initial_nonterminals_data nt)
+                                       (ParseNonTerminal _ p)
+                                     -> parse_nonterminal (G := ab_star_grammar') str ab_star_grammar') }) (only parsing).
+
+  Definition parse_with_correct'
+  : correct_parse_T.
+  Proof.
+    exists parse'.
+    exact (fun str => @parse_nonterminal_correct _ _ _ ab_star'_cdata str ab_star_grammar').
+  Defined.
+
+  Local Arguments string_dec : simpl never.
+
+  (*Definition simplified_parse_with_correct'
+  : correct_parse_T.
+  Proof.
+    pose parse_with_correct' as p.
+    unfold parse_with_correct' in p.
+    Notation "( x ; *** )" := (existT _ x _).
+    unfold parse', parse_nonterminal, parse_nonterminal_or_abort, parse_nonterminal_step, parse_productions, parse_production in p.
+    simpl in p.
+  Abort.*)
+
+  Definition simplified_parse' (str : string) : bool.
+  Proof.
+    pose (parse' str) as p.
+    unfold parse', parse_nonterminal, parse_nonterminal_or_abort, parse_nonterminal_step, parse_productions, combine_sig in p.
+    simpl in p.
+  Abort.
+End on_ab_star'.
